move LowParse.Spec.VCList.bare_serialize_vclist_correct from the .fsti to the .fst

src/lowparse/LowParse.Spec.VCList.fsti
@@ -971,7 +971,7 @@ let bare_serialize_vclist
   let un = U32.uint_to_t n in
   serialize ls un `Seq.append` serialize (serialize_nlist n s) l
 
-let bare_serialize_vclist_correct
+val bare_serialize_vclist_correct
   (min: nat)
   (max: nat { min <= max /\ max < 4294967296 } )
   (#lk: parser_kind)
@@ -983,20 +983,6 @@ let bare_serialize_vclist_correct
   (s: serializer p { k.parser_kind_subkind == Some ParserStrong } )
 : Lemma
   (serializer_correct (parse_vclist min max lp p) (bare_serialize_vclist min max ls s))
-= let prf (x: vlarray t min max)
-  : Lemma
-    (let fx = bare_serialize_vclist min max ls s x in
-      parse (parse_vclist min max lp p) fx == Some (x, Seq.length fx))
-  = let fx = bare_serialize_vclist min max ls s x in
-    parse_vclist_eq min max lp p fx;
-    let n = L.length x in
-    let un = U32.uint_to_t n in
-    let fn = serialize ls un in
-    parse_strong_prefix lp fn fx;
-    let fl = serialize (serialize_nlist n s) x in
-    assert (fl `Seq.equal` Seq.slice fx (Seq.length fn) (Seq.length fx))
-  in
-  Classical.forall_intro prf
 
 let serialize_vclist
   (min: nat)
